prove (for the most part) that generic extension of a core semantics preserves safeN. this is assuming that the extension implementation is soundly approximated by a particular extspec. the holes have to do with: 1) the use of evolve in safeN (which Lennart and I think could potentially be simplified); and 2) the safely_halted case in core semantics, which maybe is going away if we move to modeling program halt as calling a nonterminating external function "halt"?
the file sim_step_lemmas.v is step_lemmas.v modified to use core semantics as defined 
in sim.v instead of as in forward_simulations.v.  this file will go away when we're able to push 
the new core semantics through the rest of veric.

veric/sim_extensions.v
@@ -1,5 +1,5 @@
 Add LoadPath "..".
-Require Import veric.sim.
+Require Import veric.sim veric.sim_step_lemmas.
 
 Set Implicit Arguments.
 
@@ -28,11 +28,16 @@ Definition at_external' (c: corestate) :=
     | Some (f, args) => if handled f then None else Some (f, args)
     end end.
 
-Definition after_external (ret: Values.val) (c: corestate): option corestate :=
+Variable upd_globstate: C1 -> C2 -> option C2.
+
+Definition after_external' (ret: Values.val) (c: corestate): option corestate :=
   match c with (c1, c2) => 
     match after_external CS ret c1 with 
     | None => None
-    | Some c1' => Some (c1', c2)
+    | Some c1' => match upd_globstate c1' c2 with 
+                  | None => None
+                  | Some c2' => Some (c1', c2')
+                  end
     end end.
 
 Definition safely_halted (genv: G) (c: corestate): option Integers.Int.int := None. (*??*)
@@ -46,20 +51,21 @@ Variable handled_step_handled:
   handled f = true.
 
 Inductive corestep': G -> corestate -> M -> corestate -> M -> Prop :=
-| step_core: forall g c1 c2 m c1' m',
+| step_core: forall g c1 c2 m c1' c2' m',
   corestep CS g c1 m c1' m' -> 
-  corestep' g (c1, c2) m (c1', c2) m'
+  upd_globstate c1' c2 = Some c2' -> 
+  corestep' g (c1, c2) m (c1', c2') m'
 | step_extend: forall g c1 c2 m c2' m' f args ret c',
   at_external CS c1 = Some (f, args) -> 
   handled_step g f args c2 m ret c2' m' -> 
-  after_external ret (c1, c2') = Some c' -> 
+  after_external' ret (c1, c2') = Some c' -> 
   corestep' g (c1, c2) m c' m'.
 
 Program Definition extendCS := Build_CoreSemantics G corestate M D
   (@initial_mem _ _ _ _ CS)
   make_initial_core
   at_external'
-  after_external
+  after_external'
   safely_halted
   corestep' 
   _ _ _.
@@ -76,16 +82,16 @@ Variables (G C1 C2 D: Type) (CS: CompcertCoreSem G C1 D).
 Let corestate := (C1 * C2)%type.
 Variables 
   (init_extended_core : G -> Values.val -> list Values.val -> option C2)
+  (cores_related : C1 -> C2 -> Prop)
   (handled : AST.external_function -> bool)
-  (handled_step : G ->
-                  AST.external_function ->
+  (handled_step : G -> AST.external_function ->
                   list Values.val -> C2 -> mem -> Values.val -> C2 -> mem -> Prop)
   (handled_step_handled : forall (genv : G) (f : AST.external_function)
-                            (args : list Values.val) 
-                            (c2 : C2) (m : mem) (ret : Values.val) 
-                            (c2' : C2) (m' : mem),
-                          handled_step genv f args c2 m ret c2' m' ->
-                          handled f = true)
+    (args : list Values.val) 
+    (c2 : C2) (m : mem) (ret : Values.val) 
+    (c2' : C2) (m' : mem),
+    handled_step genv f args c2 m ret c2' m' ->
+    handled f = true)
   (handled_step_det : forall genv f args c2 m ret ret' c2' m' c2'' m'',
     handled_step genv f args c2 m ret c2' m' ->
     handled_step genv f args c2 m ret' c2'' m'' ->
@@ -94,8 +100,15 @@ Variables
     handled_step genv f args c2 m ret c2' m' ->
     allowed_core_modification m m').
 
+Variable upd_globstate: C1 -> C2 -> option C2.
+Variable upd_globstate_fun: 
+  forall c1 c2 c2' c2'',
+  upd_globstate c1 c2 = Some c2' -> 
+  upd_globstate c1 c2 = Some c2'' -> 
+  c2'=c2''.
+
 Definition extended_coresem :=
-  extendCS CS init_extended_core handled handled_step handled_step_handled.
+  extendCS CS init_extended_core handled upd_globstate handled_step handled_step_handled.
 
 Program Definition extendCCS := Build_CompcertCoreSem G corestate D
   extended_coresem _ _.
@@ -103,9 +116,10 @@ Next Obligation.
 inversion H; subst; inversion H0; subst.
 cut ((c1', m1) = (c1'0, m2)).
 inversion 1; subst; auto.
+specialize (upd_globstate_fun H2 H10); subst; auto.
 eapply csem_corestep_fun; eauto.
-apply corestep_not_at_external in H1; rewrite H1 in H4; congruence.
-apply corestep_not_at_external in H10; rewrite H10 in H1; congruence.
+apply corestep_not_at_external in H1; rewrite H1 in *; congruence.
+apply corestep_not_at_external in H7; rewrite H7 in *; congruence.
 rewrite H1 in H6; inversion H6; subst.
 destruct (handled_step_det H2 H8) as [H20 [H21 H22]]; subst.
 rewrite H12 in H3; inversion H3; subst; auto.
@@ -116,12 +130,130 @@ apply csem_allowed_modifications in H0; auto.
 eapply handled_step_allowed_core_modifications; eauto.
 Qed.
 
-End compcert_extension.
+(* extensions preserve safety *)
+
+Variable ora: Type.
+Variable ExtSpec: external_specification mem AST.external_function ora.
+
+Variable INV_PRE: forall ge ef args c2 m (x : ext_spec_type ExtSpec ef) z, 
+  ext_spec_pre ExtSpec ef x args c2 m ->
+  exists ret, exists c2', exists m', handled_step ge ef args z m ret c2' m'.
+
+Variable INV_POST: forall ge ef args c2 m ret c2' m' x z, 
+  ext_spec_pre ExtSpec ef x args z m -> 
+  handled_step ge ef args c2 m ret c2' m' ->
+  ext_spec_post ExtSpec ef x ret z m'. 
+
+Variable CORE_DIAGRAM_HANDLED: forall ge f args ret c1 c2 m c2' c2'' m' c1',
+  cores_related c1 c2 -> 
+  at_external CS c1 = Some (f, args) -> 
+  handled_step ge f args c2 m ret c2' m' -> 
+  after_external' CS upd_globstate ret (c1, c2') = Some (c1', c2'') -> 
+  cores_related c1' c2''.
+
+Variable CORE_DIAGRAM_UNHANDLED: forall f args ret c1 c2 c1' c2',
+  cores_related c1 c2 -> 
+  at_external CS c1 = Some (f, args) -> 
+  handled f = false -> 
+  after_external' CS upd_globstate ret (c1, c2) = Some (c1', c2') -> 
+  cores_related c1' c2'.
+
+Variable upd_after_external1: 
+  forall ef l ret c1 c2 c1',
+  cores_related c1 c2 -> 
+  at_external CS c1 = Some (ef, l) -> 
+  after_external CS ret c1 = Some c1' -> 
+  exists c2', upd_globstate c1' c2 = Some c2'.
+
+Variable upd_after_external2: 
+  forall ge ef l ret c1 c2 c1' c2' m m', 
+  cores_related c1 c2 -> 
+  at_external CS c1 = Some (ef, l) -> 
+  handled_step ge ef l c2 m ret c2' m' -> 
+  after_external CS ret c1 = Some c1' -> 
+  exists c2'', upd_globstate c1' c2' = Some c2''.
+
+Variable upd_after_corestep: 
+  forall ge c1 c2 c1' m m',
+  cores_related c1 c2 -> 
+  corestep CS ge c1 m c1' m' -> 
+  exists c2', 
+    upd_globstate c1' c2 = Some c2' /\ 
+    cores_related c1' c2'.
+
+Lemma extendCCS_safeN ge (z: ora) (c1: C1) (c2: C2) (m: mem) (n: nat) :
+  cores_related c1 c2 -> 
+  safeN CS ExtSpec ge n z c1 m -> 
+  safeN extendCCS ExtSpec ge n z (c1, c2) m.
+Proof.
+revert ge c1 c2 z m; induction n; simpl; auto.
+intros ge c1 c2 z m H1.
+case_eq (at_external CS c1).
+destruct p as [ef l].
+case_eq (handled ef).
+destruct (sim.safely_halted CS ge c1).
+intros; elimtype False; auto.
+intros H2 H3 [x H4].
+assert (H5: ext_spec_evolve ExtSpec z z) by admit. (*evolve must evolve...*)
+specialize (H4 z H5).
+destruct H4 as [H4 H7].
+destruct (INV_PRE ge ef l z m x c2 H4) as [ret [c2' [m' H8]]].
+generalize H8 as H8'.
+apply INV_POST with (z := z) (x := x) in H8.
+destruct (H7 ret m' z H8) as [c1' [H9 H10]]; intros H11.
+destruct (upd_after_external2 H1 H3 H11 H9) as [c2'' H12].
+exists (c1', c2''). 
+exists m'.
+assert (H13: after_external' CS upd_globstate ret (c1, c2') = Some (c1', c2'')).
+ unfold after_external'. 
+ rewrite H9; auto.
+ rewrite H12; auto.
+split.
+eapply step_extend; eauto.
+eapply IHn; auto.
+eapply CORE_DIAGRAM_HANDLED; eauto.
+auto.
+
+intros H2 H3.
+destruct (sim.safely_halted CS ge c1).
+inversion 1.
+intros [x H4].
+exists x.
+intros z' H5; split.
+destruct (H4 z' H5).
+auto.
+intros ret m' z'' H6.
+destruct (H4 z' H5) as [H0 H7].
+destruct (H7 _ _ _ H6) as [c1' [H9 H10]].
+destruct (upd_after_external1 _ H1 H3 H9) as [c2' H11]. 
+exists (c1', c2').
+rewrite H9.
+rewrite H11.
+split; auto.
+eapply IHn; eauto.
+eapply CORE_DIAGRAM_UNHANDLED with (ret := ret); eauto.
+unfold after_external'.
+rewrite H9.
+rewrite H11.
+split; auto.
+
+destruct (sim.safely_halted CS ge c1).
+admit. (*let's assume we're never safely halted; HALT is an external 
+         function call that never returns*)
+intros H2 [c' [m' [H3 H4]]].
+destruct (upd_after_corestep _ _ _ _ H1 H3) as [c2' [H5 H6]].
+exists (c', c2').
+exists m'.
+split.
+eapply step_core; eauto.
+eapply IHn; eauto.
+Qed.
 
 (* NOTES: 
--1) extensions preserve safety; needs axioms about safety of handled_step at external calls
 -2) preservation of simulation diagrams (probably 3 cases)
 -3) define a simple extension with one external function call; show that it satisfies 
 properties (1) and (2)
 -4) do same for concurrency extension
 *)
+
+End compcert_extension.
